separated lemmas from definitions

Formalization_Isabelle_Nicole/CommunicatingAutomaton.thy
@@ -1,109 +1,12 @@
 (* Author: Kirstin Peters, Augsburg University, 2024 *)
 
-theory CommunicatingAutomata
-  imports "HOL-Library.Sublist" FormalLanguages
+theory CommunicatingAutomaton
+  imports Defs
 
 begin
 
 section \<open>Communicating Automata\<close>
 
-subsection \<open>Messages and Actions\<close>
-
-datatype ('information, 'peer) message =
-  Message 'information 'peer 'peer  ("_\<^bsup>_\<rightarrow>_\<^esup>" [120, 120, 120] 100)
-
-primrec get_information :: "('information, 'peer) message \<Rightarrow> 'information" where
-  "get_information (i\<^bsup>p\<rightarrow>q\<^esup>) = i"
-
-primrec get_sender :: "('information, 'peer) message \<Rightarrow> 'peer" where
-  "get_sender (i\<^bsup>p\<rightarrow>q\<^esup>) = p"
-
-primrec get_receiver :: "('information, 'peer) message \<Rightarrow> 'peer" where
-  "get_receiver (i\<^bsup>p\<rightarrow>q\<^esup>) = q"
-
-value "get_information (i\<^bsup>p\<rightarrow>q\<^esup>)"
-value "get_sender (i\<^bsup>p\<rightarrow>q\<^esup>)"
-value "get_receiver (i\<^bsup>p\<rightarrow>q\<^esup>)"
-
-datatype ('information, 'peer) action =
-  Output "('information, 'peer) message"  ("!\<langle>_\<rangle>" [120] 100) |
-  Input "('information, 'peer) message"  ("?\<langle>_\<rangle>" [120] 100)
-
-primrec is_output :: "('information, 'peer) action \<Rightarrow> bool" where
-  "is_output (!\<langle>m\<rangle>) = True" |
-  "is_output (?\<langle>m\<rangle>) = False"
-
-abbreviation is_input :: "('information, 'peer) action \<Rightarrow> bool" where
-  "is_input a \<equiv> \<not>(is_output a)"
-
-primrec get_message :: "('information, 'peer) action \<Rightarrow> ('information, 'peer) message" where
-  "get_message (!\<langle>m\<rangle>) = m" |
-  "get_message (?\<langle>m\<rangle>) = m"
-
-primrec get_actor :: "('information, 'peer) action \<Rightarrow> 'peer" where
-  "get_actor (!\<langle>m\<rangle>) = get_sender m" |
-  "get_actor (?\<langle>m\<rangle>) = get_receiver m"
-
-primrec get_object :: "('information, 'peer) action \<Rightarrow> 'peer" where
-  "get_object (!\<langle>m\<rangle>) = get_receiver m" |
-  "get_object (?\<langle>m\<rangle>) = get_sender m"
-
-abbreviation get_info :: "('information, 'peer) action \<Rightarrow> 'information" where
-  "get_info a \<equiv> get_information (get_message a)"
-
-subsection \<open>Projections & Languages\<close>
-
-abbreviation projection_on_outputs
-  :: "('information, 'peer) action word \<Rightarrow> ('information, 'peer) action word"  ("_\<down>\<^sub>!" [90] 110)
-  where
-    "w\<down>\<^sub>! \<equiv> filter is_output w"
-
-abbreviation projection_on_outputs_language
-  :: "('information, 'peer) action language \<Rightarrow> ('information, 'peer) action language"
-  ("_\<downharpoonright>\<^sub>!" [120] 100)
-  where
-    "L\<downharpoonright>\<^sub>! \<equiv> {w\<down>\<^sub>! | w. w \<in> L}"
-
-abbreviation projection_on_inputs
-  :: "('information, 'peer) action word \<Rightarrow> ('information, 'peer) action word"  ("_\<down>\<^sub>?" [90] 110)
-  where
-    "w\<down>\<^sub>? \<equiv> filter is_input w"
-
-abbreviation projection_on_inputs_language
-  :: "('information, 'peer) action language \<Rightarrow> ('information, 'peer) action language"
-  ("_\<downharpoonright>\<^sub>?" [120] 100)
-  where
-    "L\<downharpoonright>\<^sub>? \<equiv> {w\<down>\<^sub>? | w. w \<in> L}"
-
-abbreviation ignore_signs
-  :: "('information, 'peer) action word \<Rightarrow> ('information, 'peer) message word"  ("_\<down>\<^sub>!\<^sub>?" [90] 110)
-  where
-    "w\<down>\<^sub>!\<^sub>? \<equiv> map get_message w"
-
-abbreviation ignore_signs_in_language
-  :: "('information, 'peer) action language \<Rightarrow> ('information, 'peer) message language"
-  ("_\<downharpoonright>\<^sub>!\<^sub>?" [90] 110) where
-  "L\<downharpoonright>\<^sub>!\<^sub>? \<equiv> {w\<down>\<^sub>!\<^sub>? | w. w \<in> L}"
-
-\<comment> \<open>projection on receives towards p and sends from p\<close>
-abbreviation projection_on_single_peer :: "('information, 'peer) action word  \<Rightarrow> 'peer \<Rightarrow> ('information, 'peer) action word"  ("_\<down>\<^sub>_" [90, 90] 110)
-  where
-    "w\<down>\<^sub>p  \<equiv> filter (\<lambda>x. get_actor x = p) w"
-
-abbreviation projection_on_single_peer_language
-  :: "('information, 'peer) action language \<Rightarrow> 'peer \<Rightarrow> ('information, 'peer) action language"
-  ("_\<downharpoonright>\<^sub>_" [90, 90] 110) where
-  "(L\<downharpoonright>\<^sub>p) \<equiv> {(w\<down>\<^sub>p) | w. w \<in> L}"
-
-abbreviation projection_on_peer_pair
-  :: "('information, 'peer) action word \<Rightarrow> 'peer \<Rightarrow> 'peer \<Rightarrow> ('information, 'peer) action word"  ("_\<down>\<^sub>{\<^sub>_\<^sub>,\<^sub>_\<^sub>}" [90, 90, 90] 110)
-  where
-    "w\<down>\<^sub>{\<^sub>p\<^sub>,\<^sub>q\<^sub>}  \<equiv> filter (\<lambda>x. (get_object x = q \<and> get_actor x = p) \<or> (get_object x = p \<and> get_actor x = q)) w"
-
-abbreviation projection_on_peer_pair_language
-  :: "('information, 'peer) action language \<Rightarrow> 'peer \<Rightarrow> 'peer \<Rightarrow> ('information, 'peer) action language"
-  ("_\<downharpoonright>\<^sub>{\<^sub>_\<^sub>,\<^sub>_\<^sub>}" [90, 90, 90] 110) where
-  "(L\<downharpoonright>\<^sub>{\<^sub>p\<^sub>,\<^sub>q\<^sub>}) \<equiv> {(w\<down>\<^sub>{\<^sub>p\<^sub>,\<^sub>q\<^sub>}) | w. w \<in> L}"
 
 subsubsection \<open>projection simplifications on words/general cases\<close>
 
@@ -266,14 +169,6 @@ shows "prefix (w\<down>\<^sub>!\<^sub>?) (w'\<down>\<^sub>!\<^sub>?)"
 
 subsection \<open>Shuffled Language\<close>
 
-inductive shuffled ::"('information, 'peer) action word \<Rightarrow> ('information, 'peer) action word \<Rightarrow> bool" where
-  (* Base case: every word shuffles to itself *)
-  refl: "shuffled w w" |
-  (* Single swap: !x?y \<rightarrow> ?y!x *)
-  swap: "\<lbrakk> is_output a; is_input b ; w = (xs @ a # b # ys) \<rbrakk> 
-         \<Longrightarrow> shuffled w (xs @ b # a # ys)" |
-  (* Transitive closure *)
-  trans: "\<lbrakk> shuffled w w'; shuffled w' w'' \<rbrakk> \<Longrightarrow> shuffled w w''"
 
 lemma shuffled_rev:
   assumes "shuffled w w'"
@@ -324,24 +219,13 @@ next
   then show ?case  using shuffled_prepend_inductive by auto
 qed
 
-(* All possible shuffles of a word *)
-definition all_shuffles :: "('information, 'peer) action word \<Rightarrow> ('information, 'peer) action word set" where
-  "all_shuffles w = {w'. shuffled w w'}"
 
-(* Shuffled language *)
-definition shuffled_lang :: "('information, 'peer) action  language \<Rightarrow> ('information, 'peer) action language" where
-  "shuffled_lang L = (\<Union>w\<in>L. all_shuffles w)"
 
 lemma shuffle_preserves_length:
   "shuffled w w' \<Longrightarrow> length w = length w'"
   by (induction rule: shuffled.induct) auto
 
-abbreviation valid_input_shuffles_of_w :: "('information, 'peer) action word \<Rightarrow> ('information, 'peer) action language" where
-  "valid_input_shuffles_of_w w \<equiv> {w'. shuffled w w'}"
 
-abbreviation valid_input_shuffle :: 
-  "('information, 'peer) action word \<Rightarrow> ('information, 'peer) action word \<Rightarrow> bool" (infixl "\<squnion>\<squnion>\<^sub>?" 60) where
-  "w' \<squnion>\<squnion>\<^sub>? w \<equiv> shuffled w w'"
 
 lemma shuffled_lang_subset_lang : 
   assumes "w \<in> L"
@@ -444,11 +328,6 @@ lemma fully_shuffled_valid_gen:
   shows "([?\<langle>(a\<^bsup>q\<rightarrow>p\<^esup>)\<rangle>] @ xs) \<squnion>\<squnion>\<^sub>? (xs @ [?\<langle>(a\<^bsup>q\<rightarrow>p\<^esup>)\<rangle>])"
   by (meson assms(2) fully_shuffled_gen)
 
-abbreviation shuffling_possible :: "('information, 'peer) action word \<Rightarrow> bool" where
-  "shuffling_possible w \<equiv> (\<exists> xs a b ys. is_output a \<and> is_input b \<and> w = (xs @ a # b # ys))"
-
-abbreviation shuffling_occurred :: "('information, 'peer) action word \<Rightarrow> bool" where
-  "shuffling_occurred w \<equiv> (\<exists> xs a b ys. is_output a \<and> is_input b \<and> w = (xs @ b # a # ys))"
 
 lemma shuffling_possible_to_existing_shuffle:
   assumes "shuffling_possible w" 
@@ -560,9 +439,6 @@ next
   qed
 qed
 
-(*w' is the result of shuffling w once, on the rightmost eligible pair*) 
-abbreviation rightmost_shuffle :: "('information, 'peer) action word \<Rightarrow> ('information, 'peer) action word \<Rightarrow> bool" where
-  "rightmost_shuffle w w' \<equiv> (\<exists> xs a b ys. is_output a \<and> is_input b \<and> w = (xs @ a # b # ys) \<and> (\<not> shuffling_possible ys) \<and> w' = (xs @ b # a # ys))"
 
 lemma rightmost_shuffle_is_shuffle:
   assumes "rightmost_shuffle v w" 
@@ -639,23 +515,7 @@ lemma shuffle_keeps_recv_order:
 
 subsection \<open>A Communicating Automaton\<close>
 
-locale CommunicatingAutomaton =
-  fixes peer        :: "'peer"
-    and States      :: "'state set"
-    and initial     :: "'state"
-    and Messages    :: "('information, 'peer) message set"
-    and Transitions :: "('state \<times> ('information, 'peer) action \<times> 'state) set"
-  assumes finite_states:          "finite States"
-    and initial_state:          "initial \<in> States"
-    and message_alphabet:       "Alphabet Messages"
-    and well_formed_transition: "\<And>s1 a s2. (s1, a, s2) \<in> Transitions \<Longrightarrow>
-                                   s1 \<in> States \<and> get_message a \<in> Messages \<and> get_actor a = peer \<and>
-                                   get_object a \<noteq> peer \<and> s2 \<in> States"
-begin
-
-inductive_set ActionsOverMessages :: "('information, 'peer) action set" where
-  AOMOutput: "m \<in> Messages \<Longrightarrow> !\<langle>m\<rangle> \<in> ActionsOverMessages" |
-  AOMInput:  "m \<in> Messages \<Longrightarrow> ?\<langle>m\<rangle> \<in> ActionsOverMessages"
+context CommunicatingAutomaton begin
 
 lemma ActionsOverMessages_rev:
   assumes "a \<in> ActionsOverMessages"
@@ -702,8 +562,6 @@ proof -
     by simp
 qed
 
-inductive_set Actions :: "('information, 'peer) action set"  ("Act") where
-  ActOfTrans: "(s1, a, s2) \<in> Transitions \<Longrightarrow> a \<in> Act"
 
 lemma Actions_rev :
   assumes "a \<in> Act"
@@ -742,9 +600,6 @@ lemma Act_is_finite:
     finite_subset[of Act ActionsOverMessages]
   by simp
 
-inductive_set CommunicationPartners :: "'peer set" where
-  CPAction: "(s1, a, s2) \<in> Transitions \<Longrightarrow> get_object a \<in> CommunicationPartners"
-
 lemma ComunicationPartners_is_finite:
   shows "finite CommunicationPartners"
 proof -
@@ -760,9 +615,6 @@ proof -
     by simp
 qed
 
-inductive_set SendingToPeers :: "'peer set" where
-  SPSend: "\<lbrakk>(s1, a, s2) \<in> Transitions; is_output a\<rbrakk> \<Longrightarrow> get_object a \<in> SendingToPeers"
-
 lemma SendingToPeers_rev:
   fixes p :: "'peer"
   assumes "p \<in> SendingToPeers"
@@ -774,9 +626,6 @@ lemma SendingToPeers_is_subset_of_CommunicationPartners:
   shows "SendingToPeers \<subseteq> CommunicationPartners"
   using CommunicationPartners.intros SendingToPeersp.simps SendingToPeersp_SendingToPeers_eq
   by auto
-
-inductive_set ReceivingFromPeers :: "'peer set" where
-  RPRecv: "\<lbrakk>(s1, a, s2) \<in> Transitions; is_input a\<rbrakk> \<Longrightarrow> get_object a \<in> ReceivingFromPeers"
 
 lemma ReceivingFromPeers_rev:
   fixes p :: "'peer"
@@ -812,21 +661,6 @@ qed
 
 
 
-abbreviation step
-  :: "'state \<Rightarrow> ('information, 'peer) action \<Rightarrow> 'state \<Rightarrow> bool"  ("_ \<midarrow>_\<rightarrow> _" [90, 90, 90] 110)
-  where
-    "s1 \<midarrow>a\<rightarrow> s2 \<equiv> (s1, a, s2) \<in> Transitions"
-
-(*
-\<comment> \<open>this is the original run def, i swapped it to (a#w) (see below)\<close>
-inductive run :: "'state \<Rightarrow> ('information, 'peer) action word \<Rightarrow> 'state list \<Rightarrow> bool" where
-REmpty:    "run s \<epsilon> ([])" |
-RComposed: "\<lbrakk>run s0 w xs; last (s0#xs) \<midarrow>a\<rightarrow> s\<rbrakk> \<Longrightarrow> run s0 (w\<cdot>[a]) (xs@[s])"
-*)
-
-inductive run :: "'state \<Rightarrow> ('information, 'peer) action word \<Rightarrow> 'state list \<Rightarrow> bool" where
-  REmpty2:    "run s \<epsilon> ([])" |
-  RComposed2: "\<lbrakk>run s1 w xs; s0 \<midarrow>a\<rightarrow> s1\<rbrakk> \<Longrightarrow> run s0 (a # w) (s1 # xs)"
 
 lemma run_rev :
   assumes "run s0 (a # w) (s1 # xs)"
@@ -891,9 +725,6 @@ next
 qed
 
 
-inductive_set Traces :: "('information, 'peer) action word set" where
-  STRun: "run initial w xs \<Longrightarrow> w \<in> Traces"
-
 lemma Traces_rev : 
   fixes w :: "('information, 'peer) action word"
   assumes "w \<in> Traces"
@@ -924,59 +755,13 @@ shows "last (s0#xs) \<midarrow>a\<rightarrow> s \<and> run s0 w xs"
   using assms run.cases by fastforce
 *)
 
-abbreviation Lang :: "('information, 'peer) action language" where
-  "Lang \<equiv> Traces"
-
-abbreviation LangSend :: "('information, 'peer) action language" where
-  "LangSend \<equiv> Lang\<downharpoonright>\<^sub>!"
-
-abbreviation LangRecv :: "('information, 'peer) action language" where
-  "LangRecv \<equiv> Lang\<downharpoonright>\<^sub>?"
-
 end
 
 subsection \<open>Network of Communicating Automata\<close>
 
-locale NetworkOfCA =
-  fixes automata :: "'peer \<Rightarrow> ('state set \<times> 'state \<times>
-                     ('state \<times> ('information, 'peer) action \<times> 'state) set)"  ("\<A>" 1000)
-    and messages :: "('information, 'peer) message set"                       ("\<M>" 1000)
-  assumes finite_peers:      "finite (UNIV :: 'peer set)"
-    and automaton_of_peer: "\<And>p. CommunicatingAutomaton p (fst (\<A> p)) (fst (snd (\<A> p))) \<M>
-                                   (snd (snd (\<A> p)))"
-    and message_alphabet:  "Alphabet \<M>"
-    and peers_of_message:  "\<And>m. m \<in> \<M> \<Longrightarrow> get_sender m \<noteq> get_receiver m"
-    and messages_used:     "\<forall>m \<in> \<M>. \<exists>s1 a s2 p. (s1, a, s2) \<in> snd (snd (\<A> p)) \<and>
-                              m = get_message a"
+context NetworkOfCA 
 begin
 
-\<comment> \<open>all peers in network\<close>
-abbreviation get_peers :: "'peer set" ("\<P>" 110) where
-  "\<P> \<equiv> (UNIV :: 'peer set)"
-
-abbreviation get_states :: "'peer \<Rightarrow> 'state set"  ("\<S> _" [90] 110) where
-  "\<S>(p) \<equiv> fst (\<A> p)"
-
-abbreviation get_initial_state :: "'peer \<Rightarrow> 'state"  ("\<I> _" [90] 110) where
-  "\<I>(p) \<equiv> fst (snd (\<A> p))"
-
-abbreviation get_transitions
-  :: "'peer \<Rightarrow> ('state \<times> ('information, 'peer) action \<times> 'state) set"  ("\<R> _" [90] 110) where
-  "\<R>(p) \<equiv> snd (snd (\<A> p))"
-
-abbreviation WordsOverMessages :: "('information, 'peer) message word set"  ("\<M>\<^sup>*" 100) where
-  "\<M>\<^sup>* \<equiv> Alphabet.WordsOverAlphabet \<M>"
-
-\<comment> \<open>all q that p sends to in Ap (for which there is a transition !p->q in Ap)\<close>
-abbreviation sendingToPeers_of_peer :: "'peer \<Rightarrow> 'peer set"  ("\<P>\<^sub>! _" [90] 110) where
-  "\<P>\<^sub>!(p) \<equiv> CommunicatingAutomaton.SendingToPeers (snd (snd (\<A> p)))"
-
-\<comment> \<open>all q that p receives from in Ap (for which there is a transition ?q->p in Ap)\<close>
-abbreviation receivingFromPeers_of_peer :: "'peer \<Rightarrow> 'peer set"  ("\<P>\<^sub>? _" [90] 110) where
-  "\<P>\<^sub>?(p) \<equiv> CommunicatingAutomaton.ReceivingFromPeers (snd (snd (\<A> p)))"
-
-abbreviation Peers_of :: "'peer \<Rightarrow> 'peer set" where
-  "Peers_of p \<equiv> CommunicatingAutomaton.CommunicationPartners (snd (snd (\<A> p)))"
 
 lemma peer_trans_to_message_in_network:
   assumes "(s1, a, s2) \<in> \<R>(p)"
@@ -990,25 +775,8 @@ term "\<A>"
 term "\<A> p"
 term "(snd (snd (\<A> p)))"
 
-abbreviation step_of_peer
-  :: "'state \<Rightarrow> ('information, 'peer) action \<Rightarrow> 'peer \<Rightarrow> 'state \<Rightarrow> bool"
-  ("_ \<midarrow>_\<rightarrow>_ _" [90, 90, 90, 90] 110) where
-  "s1 \<midarrow>a\<rightarrow>p s2 \<equiv> (s1, a, s2) \<in> snd (snd (\<A> p))"
-
-abbreviation language_of_peer
-  :: "'peer \<Rightarrow> ('information, 'peer) action language"  ("\<L> _" [90] 110) where
-  "\<L>(p) \<equiv> CommunicatingAutomaton.Lang (fst (snd (\<A> p))) (snd (snd (\<A> p)))"
-
 term "(fst (snd (\<A> p)))"
 term "(snd (snd (\<A> p)))"
-
-abbreviation output_language_of_peer
-  :: "'peer \<Rightarrow> ('information, 'peer) action language"  ("\<L>\<^sub>! _" [90] 110) where
-  "\<L>\<^sub>!(p) \<equiv> CommunicatingAutomaton.LangSend (fst (snd (\<A> p))) (snd (snd (\<A> p)))"
-
-abbreviation input_language_of_peer
-  :: "'peer \<Rightarrow> ('information, 'peer) action language"  ("\<L>\<^sub>? _" [90] 110) where
-  "\<L>\<^sub>?(p) \<equiv> CommunicatingAutomaton.LangRecv (fst (snd (\<A> p))) (snd (snd (\<A> p)))"
 
 
 subsection \<open>helpful conclusions about language/ runs / etc. in concrete cases and peer runs\<close>
@@ -1175,24 +943,6 @@ proof -
   then show ?thesis by (meson CommunicatingAutomaton.Traces.intros automaton_of_peer)
 qed
 
-  \<comment> \<open>start in s1, read w (in 0 or more steps) and end in s2 \<close>  
-abbreviation path_of_peer
-  :: "'state \<Rightarrow> ('information, 'peer) action word \<Rightarrow> 'peer \<Rightarrow> 'state \<Rightarrow> bool"
-  ("_ \<midarrow>_\<rightarrow>\<^sup>*_ _" [90, 90, 90, 90] 110) where
-  "s1 \<midarrow>w\<rightarrow>\<^sup>*p s2 \<equiv> (s1=s2 \<and> w = \<epsilon> \<and> s1 \<in> \<S> p)  \<or> (\<exists>xs. CommunicatingAutomaton.run (\<R> p) s1 w xs \<and> last xs = s2)"
-
-abbreviation run_of_peer
-  :: " 'peer \<Rightarrow> ('information, 'peer) action word \<Rightarrow> 'state  list \<Rightarrow> bool" where
-  "run_of_peer p w xs \<equiv> (CommunicatingAutomaton.run (\<R> p) (\<I> p) w xs)"
-
-abbreviation run_of_peer_from_state
-  :: " 'peer \<Rightarrow> 'state \<Rightarrow> ('information, 'peer) action word \<Rightarrow> 'state  list \<Rightarrow> bool" where
-  "run_of_peer_from_state p s w xs \<equiv> (CommunicatingAutomaton.run (\<R> p) s w xs)"
-
-fun get_trans_of_run :: "'state \<Rightarrow> ('information, 'peer) action word \<Rightarrow> 'state list \<Rightarrow> ('state \<times> ('information, 'peer) action \<times> 'state) list" where
-  "get_trans_of_run s0 \<epsilon> [] = []" |
-  "get_trans_of_run s0 [a] [s1] = [(s0, a, s1)]" |
-  "get_trans_of_run s0 (a # as) (s1 # xs) = (s0, a, s1) # get_trans_of_run s1 as xs"
 
 
 lemma lang_implies_run_alt :
@@ -1334,11 +1084,6 @@ qed
 
 subsection \<open>Synchronous System\<close>
 
-definition is_sync_config :: "('peer \<Rightarrow> 'state) \<Rightarrow> bool" where
-  "is_sync_config C \<equiv> (\<forall>p. C p \<in> \<S>(p))"
-
-abbreviation initial_sync_config :: "'peer \<Rightarrow> 'state"  ("\<C>\<^sub>\<I>\<^sub>\<zero>") where
-  "\<C>\<^sub>\<I>\<^sub>\<zero> \<equiv> \<lambda>p. \<I>(p)"
 
 lemma initial_configuration_is_synchronous_configuration:
   shows "is_sync_config \<C>\<^sub>\<I>\<^sub>\<zero>"
@@ -1351,11 +1096,6 @@ proof clarify
     by simp
 qed
 
-inductive sync_step
-  :: "('peer \<Rightarrow> 'state) \<Rightarrow> ('information, 'peer) action \<Rightarrow> ('peer \<Rightarrow> 'state) \<Rightarrow> bool"
-  ("_ \<midarrow>\<langle>_, \<zero>\<rangle>\<rightarrow> _" [90, 90, 90] 110) where
-  SynchStep: "\<lbrakk>is_sync_config C1; a = !\<langle>(i\<^bsup>p\<rightarrow>q\<^esup>)\<rangle>; C1 p \<midarrow>!\<langle>(i\<^bsup>p\<rightarrow>q\<^esup>)\<rangle>\<rightarrow>p (C2 p);
-             C1 q \<midarrow>?\<langle>(i\<^bsup>p\<rightarrow>q\<^esup>)\<rangle>\<rightarrow>q (C2 q); \<forall>x. x \<notin> {p, q} \<longrightarrow> C1(x) = C2(x)\<rbrakk> \<Longrightarrow> C1 \<midarrow>\<langle>a, \<zero>\<rangle>\<rightarrow> C2"
 
 lemma sync_step_rev:
   fixes C1 C2 :: "'peer \<Rightarrow> 'state"
@@ -1363,7 +1103,7 @@ lemma sync_step_rev:
   assumes "C1 \<midarrow>\<langle>a, \<zero>\<rangle>\<rightarrow> C2"
   shows "is_sync_config C1" and "is_sync_config C2" and "\<exists>i p q. a = !\<langle>(i\<^bsup>p\<rightarrow>q\<^esup>)\<rangle>"
     and "get_actor a \<noteq> get_object a" and "C1 (get_actor a) \<midarrow>a\<rightarrow>(get_actor a) (C2 (get_actor a))"
-    and "\<exists>m. a = !\<langle>m\<rangle> \<and> C1 (get_object a) \<midarrow>?\<langle>m\<rangle>\<rightarrow>(get_object a) (C2 (get_object a))"
+    and "\<exists>m. a = !\<langle>m\<rangle> \<and> C1 (get_object a) \<midarrow>(?\<langle>m\<rangle>)\<rightarrow>(get_object a) (C2 (get_object a))"
     and "\<forall>x. x \<notin> {get_actor a, get_object a} \<longrightarrow> C1(x) = C2(x)"
   using assms
 proof induct
@@ -1373,7 +1113,7 @@ proof induct
   assume A2: "a = !\<langle>(i\<^bsup>p\<rightarrow>q\<^esup>)\<rangle>"
   thus "\<exists>i p q. a = !\<langle>(i\<^bsup>p\<rightarrow>q\<^esup>)\<rangle>"
     by blast
-  assume A3: "C1 p \<midarrow>!\<langle>(i\<^bsup>p\<rightarrow>q\<^esup>)\<rangle>\<rightarrow>p (C2 p)"
+  assume A3: "C1 p \<midarrow>(!\<langle>(i\<^bsup>p\<rightarrow>q\<^esup>)\<rangle>)\<rightarrow>p (C2 p)"
   with A2 show "C1 (get_actor a) \<midarrow>a\<rightarrow>(get_actor a) (C2 (get_actor a))"
     by simp
   have A4: "CommunicatingAutomaton p (\<S> p) (\<I> p) \<M> (\<R> p)"
@@ -1382,8 +1122,8 @@ proof induct
   with A2 A3 show "get_actor a \<noteq> get_object a"
     using CommunicatingAutomaton.well_formed_transition[of p "\<S> p" "\<I> p" \<M> "\<R> p" "C1 p" a "C2 p"]
     by auto
-  assume A5: "C1 q \<midarrow>?\<langle>(i\<^bsup>p\<rightarrow>q\<^esup>)\<rangle>\<rightarrow>q (C2 q)"
-  with A2 show "\<exists>m. a = !\<langle>m\<rangle> \<and> C1 (get_object a) \<midarrow>?\<langle>m\<rangle>\<rightarrow>(get_object a) (C2 (get_object a))"
+  assume A5: "C1 q \<midarrow>(?\<langle>(i\<^bsup>p\<rightarrow>q\<^esup>)\<rangle>)\<rightarrow>q (C2 q)"
+  with A2 show "\<exists>m. a = !\<langle>m\<rangle> \<and> C1 (get_object a) \<midarrow>(?\<langle>m\<rangle>)\<rightarrow>(get_object a) (C2 (get_object a))"
     by auto
   assume A6: "\<forall>x. x \<notin> {p, q} \<longrightarrow> C1 x = C2 x"
   with A2 show "\<forall>x. x \<notin> {get_actor a, get_object a} \<longrightarrow> C1(x) = C2(x)"
@@ -1424,16 +1164,11 @@ lemma sync_step_output_rev:
     and i     :: "'information"
     and p q   :: "'peer"
   assumes "C1 \<midarrow>\<langle>!\<langle>(i\<^bsup>p\<rightarrow>q\<^esup>)\<rangle>, \<zero>\<rangle>\<rightarrow> C2"
-  shows "is_sync_config C1" and "is_sync_config C2" and "p \<noteq> q" and "C1 p \<midarrow>!\<langle>(i\<^bsup>p\<rightarrow>q\<^esup>)\<rangle>\<rightarrow>p (C2 p)"
-    and "C1 q \<midarrow>?\<langle>(i\<^bsup>p\<rightarrow>q\<^esup>)\<rangle>\<rightarrow>q (C2 q)" and "\<forall>x. x \<notin> {p, q} \<longrightarrow> C1(x) = C2(x)"
+  shows "is_sync_config C1" and "is_sync_config C2" and "p \<noteq> q" and "C1 p \<midarrow>(!\<langle>(i\<^bsup>p\<rightarrow>q\<^esup>)\<rangle>)\<rightarrow>p (C2 p)"
+    and "C1 q \<midarrow>(?\<langle>(i\<^bsup>p\<rightarrow>q\<^esup>)\<rangle>)\<rightarrow>q (C2 q)" and "\<forall>x. x \<notin> {p, q} \<longrightarrow> C1(x) = C2(x)"
   using assms sync_step_rev[of C1 "!\<langle>(i\<^bsup>p\<rightarrow>q\<^esup>)\<rangle>" C2]
   by simp_all
 
-inductive sync_run
-  :: "('peer \<Rightarrow> 'state) \<Rightarrow> ('information, 'peer) action word \<Rightarrow> ('peer \<Rightarrow> 'state) list \<Rightarrow> bool"
-  where
-    SREmpty:    "sync_run C \<epsilon> ([])" |
-    SRComposed: "\<lbrakk>sync_run C0 w xc; last (C0#xc) \<midarrow>\<langle>a, \<zero>\<rangle>\<rightarrow> C\<rbrakk> \<Longrightarrow> sync_run C0 (w\<cdot>[a]) (xc@[C])"
 
 lemma sync_run_rev :
   assumes "sync_run C0 (w\<cdot>[a]) (xc@[C])"
@@ -1511,18 +1246,11 @@ next
 qed
 *)
 
-\<comment> \<open>E(Nsync)\<close>
-inductive_set SyncTraces :: "('information, 'peer) action language"  ("\<T>\<^sub>\<zero>" 120) where
-  STRun: "sync_run \<C>\<^sub>\<I>\<^sub>\<zero> w xc \<Longrightarrow> w \<in> \<T>\<^sub>\<zero>"
 
 lemma SyncTraces_rev :
   assumes "w \<in> \<T>\<^sub>\<zero>"
   shows "\<exists>xc. sync_run \<C>\<^sub>\<I>\<^sub>\<zero> w xc"
   using SyncTraces.simps assms by auto
-
-\<comment> \<open>T(Nsync)\<close>
-abbreviation SyncLang :: "('information, 'peer) action language"  ("\<L>\<^sub>\<zero>" 120) where
-  "\<L>\<^sub>\<zero> \<equiv> \<T>\<^sub>\<zero>"
 
 lemma no_inputs_in_synchronous_communication:
   shows "\<L>\<^sub>\<zero>\<downharpoonright>\<^sub>! = \<L>\<^sub>\<zero>" and "\<L>\<^sub>\<zero>\<downharpoonright>\<^sub>? \<subseteq> {\<epsilon>}"
@@ -1541,7 +1269,7 @@ qed
 
 lemma sync_send_step_to_recv_step: 
   assumes "C1 \<midarrow>\<langle>!\<langle>(i\<^bsup>p\<rightarrow>q\<^esup>)\<rangle>, \<zero>\<rangle>\<rightarrow> C2"
-  shows "C1 q \<midarrow>?\<langle>(i\<^bsup>p\<rightarrow>q\<^esup>)\<rangle>\<rightarrow>q (C2 q)"
+  shows "C1 q \<midarrow>(?\<langle>(i\<^bsup>p\<rightarrow>q\<^esup>)\<rangle>)\<rightarrow>q (C2 q)"
   using assms sync_step_output_rev(5) by auto
 
 lemma act_in_sync_word_to_sync_step: 
@@ -1551,7 +1279,7 @@ lemma act_in_sync_word_to_sync_step:
 
 lemma act_in_sync_word_to_matching_peer_steps: 
   assumes "w \<in> \<L>\<^sub>\<zero>" and "(!\<langle>(i\<^bsup>p\<rightarrow>q\<^esup>)\<rangle>) \<in> set w"
-  shows "\<exists>C1 C2. C1 p \<midarrow>!\<langle>(i\<^bsup>p\<rightarrow>q\<^esup>)\<rangle>\<rightarrow>p (C2 p) \<and> C1 q \<midarrow>?\<langle>(i\<^bsup>p\<rightarrow>q\<^esup>)\<rangle>\<rightarrow>q (C2 q)"
+  shows "\<exists>C1 C2. C1 p \<midarrow>(!\<langle>(i\<^bsup>p\<rightarrow>q\<^esup>)\<rangle>)\<rightarrow>p (C2 p) \<and> C1 q \<midarrow>(?\<langle>(i\<^bsup>p\<rightarrow>q\<^esup>)\<rangle>)\<rightarrow>q (C2 q)"
   using act_in_sync_word_to_sync_step assms(1,2) sync_send_step_to_recv_step sync_step_output_rev(4)
   by blast
 
@@ -1582,18 +1310,6 @@ subsection \<open>Mailbox System\<close>
 
 subsubsection \<open>Semantics and Language\<close>
 
-definition is_mbox_config
-  :: "('peer \<Rightarrow> ('state \<times> ('information, 'peer) message word)) \<Rightarrow> bool" where
-  "is_mbox_config C \<equiv> (\<forall>p. fst (C p) \<in> \<S>(p) \<and> snd (C p) \<in> \<M>\<^sup>*)"
-
-\<comment> \<open>all mbox configurations of system\<close>
-abbreviation mbox_configs 
-  :: "('peer \<Rightarrow> 'state \<times> ('information, 'peer) message list) set"  ("\<C>\<^sub>\<mm>") where
-  "\<C>\<^sub>\<mm> \<equiv> {C | C. is_mbox_config C}"
-
-abbreviation initial_mbox_config
-  :: "'peer \<Rightarrow> ('state \<times> ('information, 'peer) message word)"  ("\<C>\<^sub>\<I>\<^sub>\<mm>") where
-  "\<C>\<^sub>\<I>\<^sub>\<mm> \<equiv> \<lambda>p. (\<I> p, \<epsilon>)"
 
 lemma initial_mbox_alt :
   shows "(\<forall>p. \<C>\<^sub>\<I>\<^sub>\<mm> p = (\<C>\<^sub>\<I>\<^sub>\<zero> p, \<epsilon>))"
@@ -1610,9 +1326,6 @@ proof clarify
     by simp
 qed
 
-definition is_stable
-  :: "('peer \<Rightarrow> ('state \<times> ('information, 'peer) message word)) \<Rightarrow> bool" where
-  "is_stable C \<equiv> is_mbox_config C \<and> (\<forall>p. snd (C p) = \<epsilon>)"
 
 lemma initial_configuration_is_stable:
   shows "is_stable \<C>\<^sub>\<I>\<^sub>\<mm>"
@@ -1624,29 +1337,6 @@ lemma sync_config_to_mbox :
   shows "\<exists>C'. is_mbox_config C' \<and> C' = (\<lambda>p. (C p, \<epsilon>))"
   using assms initial_configuration_is_mailbox_configuration is_mbox_config_def
     is_sync_config_def by auto
-
-type_synonym bound = "nat option"
-
-abbreviation nat_bound :: "nat \<Rightarrow> bound"  ("\<B> _" [90] 110) where
-  "\<B> k \<equiv> Some k"
-
-abbreviation unbounded :: "bound"  ("\<infinity>" 100) where
-  "\<infinity> \<equiv> None"
-
-primrec is_bounded :: "nat \<Rightarrow> bound \<Rightarrow> bool"  ("_ <\<^sub>\<B> _" [90, 90] 110) where
-  "n <\<^sub>\<B> \<infinity> = True" |
-  "n <\<^sub>\<B> \<B> k = (n < k)"
-
-inductive mbox_step
-  :: "('peer \<Rightarrow> ('state \<times> ('information, 'peer) message word)) \<Rightarrow> ('information, 'peer) action \<Rightarrow>
-      bound \<Rightarrow> ('peer \<Rightarrow> ('state \<times> ('information, 'peer) message word)) \<Rightarrow> bool" where
-  MboxSend: "\<lbrakk>is_mbox_config C1; a = !\<langle>(i\<^bsup>p\<rightarrow>q\<^esup>)\<rangle>; fst (C1 p) \<midarrow>!\<langle>(i\<^bsup>p\<rightarrow>q\<^esup>)\<rangle>\<rightarrow>p (fst (C2 p));
-            snd (C1 p) = snd (C2 p); ( | (snd (C1 q)) | ) <\<^sub>\<B> k;
-            C2 q = (fst (C1 q), (snd (C1 q)) \<cdot> [(i\<^bsup>p\<rightarrow>q\<^esup>)]); \<forall>x. x \<notin> {p, q} \<longrightarrow> C1(x) = C2(x)\<rbrakk> \<Longrightarrow>
-            mbox_step C1 a k C2" |
-  MboxRecv: "\<lbrakk>is_mbox_config C1; a = ?\<langle>(i\<^bsup>p\<rightarrow>q\<^esup>)\<rangle>; fst (C1 q) \<midarrow>?\<langle>(i\<^bsup>p\<rightarrow>q\<^esup>)\<rangle>\<rightarrow>q (fst (C2 q));
-            (snd (C1 q)) = [(i\<^bsup>p\<rightarrow>q\<^esup>)] \<cdot> snd (C2 q); \<forall>x. x \<noteq> q \<longrightarrow> C1(x) = C2(x)\<rbrakk> \<Longrightarrow>
-            mbox_step C1 a k C2"
 
 
 lemma mbox_step_rev:
@@ -1672,7 +1362,7 @@ proof induct
   assume A2: "a = !\<langle>(i\<^bsup>p\<rightarrow>q\<^esup>)\<rangle>"
   thus "\<exists>i p q. a = !\<langle>(i\<^bsup>p\<rightarrow>q\<^esup>)\<rangle> \<or> a = ?\<langle>(i\<^bsup>p\<rightarrow>q\<^esup>)\<rangle>"
     by blast
-  assume A3: "fst (C1 p) \<midarrow>!\<langle>(i\<^bsup>p\<rightarrow>q\<^esup>)\<rangle>\<rightarrow>p (fst (C2 p))"
+  assume A3: "fst (C1 p) \<midarrow>(!\<langle>(i\<^bsup>p\<rightarrow>q\<^esup>)\<rangle>)\<rightarrow>p (fst (C2 p))"
   with A2 show "fst (C1 (get_actor a)) \<midarrow>a\<rightarrow>(get_actor a) (fst (C2 (get_actor a)))"
     by simp
   have A4: "CommunicatingAutomaton p (\<S> p) (\<I> p) \<M> (\<R> p)"
@@ -1749,7 +1439,7 @@ next
   assume A2: "a = ?\<langle>(i\<^bsup>p\<rightarrow>q\<^esup>)\<rangle>"
   thus "\<exists>i p q. a = !\<langle>(i\<^bsup>p\<rightarrow>q\<^esup>)\<rangle> \<or> a = ?\<langle>(i\<^bsup>p\<rightarrow>q\<^esup>)\<rangle>"
     by blast
-  assume A3: "fst (C1 q) \<midarrow>?\<langle>(i\<^bsup>p\<rightarrow>q\<^esup>)\<rangle>\<rightarrow>q (fst (C2 q))"
+  assume A3: "fst (C1 q) \<midarrow>(?\<langle>(i\<^bsup>p\<rightarrow>q\<^esup>)\<rangle>)\<rightarrow>q (fst (C2 q))"
   with A2 show "fst (C1 (get_actor a)) \<midarrow>a\<rightarrow>(get_actor a) (fst (C2 (get_actor a)))"
     by simp
   have A4: "CommunicatingAutomaton q (\<S> q) (\<I> q) \<M> (\<R> q)"
@@ -1826,7 +1516,7 @@ proof -
   show "p \<noteq> q"
     using assms mbox_step_rev(4)[of C1 "!\<langle>(i\<^bsup>p\<rightarrow>q\<^esup>)\<rangle>" k C2]
     by simp
-  show "fst (C1 p) \<midarrow>!\<langle>(i\<^bsup>p\<rightarrow>q\<^esup>)\<rangle>\<rightarrow>p (fst (C2 p))"
+  show "fst (C1 p) \<midarrow>(!\<langle>(i\<^bsup>p\<rightarrow>q\<^esup>)\<rangle>)\<rightarrow>p (fst (C2 p))"
     using assms mbox_step_rev(5)[of C1 "!\<langle>(i\<^bsup>p\<rightarrow>q\<^esup>)\<rangle>" k C2]
     by simp
   show "snd (C1 p) = snd (C2 p)"
@@ -1850,23 +1540,12 @@ lemma mbox_step_input_rev:
     and k     :: "bound"
   assumes "mbox_step C1 (?\<langle>(i\<^bsup>p\<rightarrow>q\<^esup>)\<rangle>) k C2"
   shows "is_mbox_config C1" and "is_mbox_config C2" and "p \<noteq> q"
-    and "fst (C1 q) \<midarrow>?\<langle>(i\<^bsup>p\<rightarrow>q\<^esup>)\<rangle>\<rightarrow>q (fst (C2 q))" and "(snd (C1 q)) = [i\<^bsup>p\<rightarrow>q\<^esup>] \<cdot> snd (C2 q)"
+    and "fst (C1 q) \<midarrow>(?\<langle>(i\<^bsup>p\<rightarrow>q\<^esup>)\<rangle>)\<rightarrow>q (fst (C2 q))" and "(snd (C1 q)) = [i\<^bsup>p\<rightarrow>q\<^esup>] \<cdot> snd (C2 q)"
     and "\<forall>x. x \<noteq> q \<longrightarrow> C1(x) = C2(x)"
   using assms mbox_step_rev[of C1 "?\<langle>(i\<^bsup>p\<rightarrow>q\<^esup>)\<rangle>" k C2]
   by simp_all
 
 
-abbreviation mbox_step_bounded
-  :: "('peer \<Rightarrow> ('state \<times> ('information, 'peer) message word)) \<Rightarrow> ('information, 'peer) action \<Rightarrow>
-      nat \<Rightarrow> ('peer \<Rightarrow> ('state \<times> ('information, 'peer) message word)) \<Rightarrow> bool"
-  ("_ \<midarrow>\<langle>_, _\<rangle>\<rightarrow> _" [90, 90, 90, 90] 110) where
-  "C1 \<midarrow>\<langle>a, n\<rangle>\<rightarrow> C2 \<equiv> mbox_step C1 a (Some n) C2"
-
-abbreviation mbox_step_unbounded
-  :: "('peer \<Rightarrow> ('state \<times> ('information, 'peer) message word)) \<Rightarrow> ('information, 'peer) action \<Rightarrow>
-      ('peer \<Rightarrow> ('state \<times> ('information, 'peer) message word)) \<Rightarrow> bool"
-  ("_ \<midarrow>\<langle>_, \<infinity>\<rangle>\<rightarrow> _" [90, 90, 90] 110) where
-  "C1 \<midarrow>\<langle>a, \<infinity>\<rangle>\<rightarrow> C2 \<equiv> mbox_step C1 a None C2"
 
 \<comment> \<open>if mbox can take a bounded step, it can also take an unbounded step\<close>
 lemma mbox_step_inclusion :
@@ -1967,15 +1646,6 @@ qed
 
 subsubsection "mbox run"
 
-inductive mbox_run
-  :: "('peer \<Rightarrow> ('state \<times> ('information, 'peer) message word)) \<Rightarrow> bound \<Rightarrow>
-      ('information, 'peer) action word \<Rightarrow>
-      ('peer \<Rightarrow> ('state \<times> ('information, 'peer) message word)) list \<Rightarrow> bool" where
-  MREmpty:       "mbox_run C k \<epsilon> ([])" |
-  MRComposedNat: "\<lbrakk>mbox_run C0 (Some k) w xc; last (C0#xc) \<midarrow>\<langle>a, k\<rangle>\<rightarrow> C\<rbrakk> \<Longrightarrow>
-                mbox_run C0 (Some k) (w\<cdot>[a]) (xc@[C])" |
-  MRComposedInf: "\<lbrakk>mbox_run C0 None w xc; last (C0#xc) \<midarrow>\<langle>a, \<infinity>\<rangle>\<rightarrow> C\<rbrakk> \<Longrightarrow>
-                mbox_run C0 None (w\<cdot>[a]) (xc@[C])"
 
 lemma mbox_run_rev_unbound :
   assumes "mbox_run C0 None (w\<cdot>[a]) (xc@[C])"
@@ -2043,11 +1713,6 @@ lemma mbox_step_to_run:
   by (metis MRComposedInf MREmpty append.left_neutral assms last_ConsL)
 
 subsubsection "mbox traces"
-\<comment> \<open>E(mbox)\<close>
-inductive_set MboxTraces
-  :: "nat option \<Rightarrow> ('information, 'peer) action language"  ("\<T>\<^bsub>_\<^esub>" [100] 120)
-  for k :: "nat option" where
-    MTRun: "mbox_run \<C>\<^sub>\<I>\<^sub>\<mm> k w xc \<Longrightarrow> w \<in> \<T>\<^bsub>k\<^esub>"
 
 lemma Mbox_Traces_rev :
   assumes "w \<in> \<T>\<^bsub>k\<^esub>"
@@ -2073,24 +1738,6 @@ lemma mbox_bounded_lang_inclusion :
   shows "\<T>\<^bsub>(Some k)\<^esub> \<subseteq> \<T>\<^bsub>None\<^esub>"
   using MboxTraces_def MboxTracesp.simps mbox_run_inclusion by fastforce
 
-\<comment> \<open>T(mbox)\<close>
-abbreviation MboxLang :: "bound \<Rightarrow> ('information, 'peer) action language"  ("\<L>\<^bsub>_\<^esub>" [100] 120)
-  where
-    "\<L>\<^bsub>k\<^esub> \<equiv> { w\<down>\<^sub>! | w. w \<in> \<T>\<^bsub>k\<^esub> }"
-
-abbreviation MboxLang_bounded_by_one :: "('information, 'peer) action language"  ("\<L>\<^sub>\<one>" 120) where
-  "\<L>\<^sub>\<one> \<equiv> \<L>\<^bsub>\<B> 1\<^esub>"
-
-abbreviation MboxLang_unbounded :: "('information, 'peer) action language"  ("\<L>\<^sub>\<infinity>" 120) where
-  "\<L>\<^sub>\<infinity> \<equiv> \<L>\<^bsub>\<infinity>\<^esub>"
-
-abbreviation MboxLangSend :: "bound \<Rightarrow> ('information, 'peer) action language"  ("\<L>\<^sub>!\<^bsub>_\<^esub>" [100] 120)
-  where
-    "\<L>\<^sub>!\<^bsub>k\<^esub> \<equiv> (\<L>\<^bsub>k\<^esub>)\<downharpoonright>\<^sub>!"
-
-abbreviation MboxLangRecv :: "bound \<Rightarrow> ('information, 'peer) action language"  ("\<L>\<^sub>?\<^bsub>_\<^esub>" [100] 120)
-  where
-    "\<L>\<^sub>?\<^bsub>k\<^esub> \<equiv> (\<L>\<^bsub>k\<^esub>)\<downharpoonright>\<^sub>?"
 
 lemma execution_implies_mbox_trace :
   assumes "w \<in> \<T>\<^bsub>k\<^esub>"
@@ -2278,15 +1925,6 @@ lemma eps_in_mbox_execs: "\<epsilon> \<in> \<T>\<^bsub>None\<^esub>" using MREmp
 
 section \<open>Synchronisability\<close>
 
-abbreviation is_synchronisable :: "bool" where
-  "is_synchronisable \<equiv> \<L>\<^sub>\<infinity> = \<L>\<^sub>\<zero>"
-
-type_synonym 'a topology = "('a \<times> 'a) set"
-
-\<comment> \<open>the topology graph of all peers\<close>
-inductive_set Edges :: "'peer topology"  ("\<G>" 110) where
-  TEdge: "i\<^bsup>p\<rightarrow>q\<^esup> \<in> \<M> \<Longrightarrow> (p, q) \<in> \<G>"
-
 lemma Edges_rev:
   fixes e :: "'peer \<times> 'peer"
   assumes "e \<in> \<G>"
@@ -2322,19 +1960,10 @@ next
     by (simp add: \<open>v\<down>\<^sub>p = v\<close> w_def)
 qed
 
-abbreviation Successors :: "'peer topology \<Rightarrow> 'peer \<Rightarrow> 'peer set"  ("_\<langle>_\<rightarrow>\<rangle>" [90, 90] 110) where
-  "E\<langle>p\<rightarrow>\<rangle> \<equiv> {q. (p, q) \<in> E}"
-
-abbreviation Predecessors :: "'peer topology \<Rightarrow> 'peer \<Rightarrow> 'peer set"  ("_\<langle>\<rightarrow>_\<rangle>" [90, 90] 110) where
-  "E\<langle>\<rightarrow>q\<rangle> \<equiv> {p. (p, q) \<in> E}"
 
 subsection \<open>Synchronisability is Deciable for Tree Topology in Mailbox Communication\<close>
 
 subsubsection \<open>Topology is a Tree\<close>
-
-inductive is_tree :: "'peer set \<Rightarrow> 'peer topology \<Rightarrow> bool" where
-  ITRoot: "is_tree {p} {}" |
-  ITNode: "\<lbrakk>is_tree P E; p \<in> P; q \<notin> P\<rbrakk> \<Longrightarrow> is_tree (insert q P) (insert (p, q) E)"
 
 lemma is_tree_rev:
   assumes "is_tree P E"
@@ -2516,8 +2145,6 @@ next
   qed  
 qed
 
-abbreviation tree_topology :: "bool" where
-  "tree_topology \<equiv> is_tree (UNIV :: 'peer set) (\<G>)"
 
 \<comment> \<open>P? is defined on each automaton p, G is the topology graph\<close>
 \<comment> \<open>This means there may be P?(p) = {} but p \<in> P!(q), thus (q,p) \<in> \<G> and q \<in> \<G>\<langle>\<rightarrow>p\<rangle>, but q \<notin> {}\<close>
@@ -2605,15 +2232,6 @@ next
   then show "False"  using Edges.simps assms(1) trans_to_edge by fastforce
 qed
 
-abbreviation is_root_from_topology :: "'peer \<Rightarrow> bool" where
-  "is_root_from_topology p \<equiv> (tree_topology \<and> \<G>\<langle>\<rightarrow>p\<rangle> = {})"
-
-abbreviation is_root_from_local :: "'peer \<Rightarrow> bool"  where
-  "is_root_from_local p \<equiv> tree_topology \<and> \<P>\<^sub>?(p) = {} \<and> (\<forall>q. p \<notin> \<P>\<^sub>!(q))"
-
-abbreviation is_root :: "'peer \<Rightarrow> bool"  where
-  "is_root p \<equiv> is_root_from_local p \<or> is_root_from_topology p"
-  (*tree_topology \<and> ((\<P>\<^sub>?(p) = {} \<and> (\<forall>q. p \<notin> \<P>\<^sub>!(q))) \<or> \<G>\<langle>\<rightarrow>p\<rangle> = {})*)
 
 lemma edge_impl_psend_or_qrecv:
   assumes "\<G>\<langle>\<rightarrow>p\<rangle> = {q}" and "tree_topology"
@@ -2684,14 +2302,6 @@ next
   then show ?thesis using assms edge_impl_psend_or_qrecv by blast
 qed
 
-abbreviation is_node_from_topology :: "'peer \<Rightarrow> bool" where
-  "is_node_from_topology p \<equiv> (tree_topology \<and> (\<exists>q. \<G>\<langle>\<rightarrow>p\<rangle> = {q}))"
-
-abbreviation is_node_from_local :: "'peer \<Rightarrow> bool"  where
-  "is_node_from_local p \<equiv> tree_topology \<and> (\<exists>q. \<P>\<^sub>?(p) = {q} \<or> p \<in> \<P>\<^sub>!(q))"
-
-abbreviation is_node :: "'peer \<Rightarrow> bool"  where
-  "is_node p \<equiv> is_node_from_topology p \<or> is_node_from_local p"
 
 lemma root_defs_eq:
   shows "is_root_from_topology p = is_root_from_local p"
@@ -2738,9 +2348,6 @@ lemma node_defs_eq:
 
 subsubsection "parent-child relationship in tree"
 
-(*q is parent of p*)
-inductive is_parent_of :: "'peer \<Rightarrow> 'peer \<Rightarrow> bool" where
-  node_parent : "\<lbrakk>is_node p; \<G>\<langle>\<rightarrow>p\<rangle> = {q}\<rbrakk> \<Longrightarrow> is_parent_of p q"
 
 lemma is_parent_of_rev:
   assumes "is_parent_of p q"
@@ -2896,10 +2503,6 @@ qed
 
 subsubsection "path to root and path related lemmas"
 
-inductive path_to_root :: "'peer \<Rightarrow> 'peer list \<Rightarrow> bool" where
-  PTRRoot: "\<lbrakk>is_root p\<rbrakk> \<Longrightarrow> path_to_root p [p]" |
-  PTRNode: "\<lbrakk>tree_topology; is_parent_of p q; path_to_root q as; distinct (p # as)\<rbrakk> \<Longrightarrow> path_to_root p (p # as)"
-
 lemma path_to_root_rev:
   assumes "path_to_root p ps" and "ps \<noteq> [p]"
   shows "\<exists>q as. is_parent_of p q \<and> path_to_root q as \<and> ps = (p # as) \<and> distinct (p # as)"
@@ -2910,8 +2513,6 @@ lemma path_to_root_rev_empty:
   assumes "path_to_root p ps" and "ps = [p]"
   shows "is_root p"
   by (metis (no_types, lifting) assms(1,2) list.distinct(1) list.inject path_to_root.simps)
-
-definition get_root :: "'peer topology \<Rightarrow> 'peer" where "get_root E = (THE x. is_root x)"
 
 lemma path_ends_at_root:
   assumes "path_to_root p ps"
@@ -2930,8 +2531,6 @@ lemma single_path_impl_root:
   shows "is_root p"
   using assms path_to_root_rev_empty by blast
 
-abbreviation get_path_to_root :: "'peer \<Rightarrow>  'peer list" where
-  "get_path_to_root p \<equiv>  (THE ps. path_to_root p ps)"
 
 lemma path_to_root_first_elem_is_peer: 
   assumes  "path_to_root p (x # ps)" 
@@ -3174,9 +2773,6 @@ next
   then show ?case using \<open>is_tree (\<P>) (\<G>) \<and> is_parent_of p x \<and> path_to_root x (x # as)\<close> path_to_root.PTRNode by blast
 qed
 
-inductive path_from_root :: "'peer \<Rightarrow> 'peer list \<Rightarrow> bool" where
-  PFRRoot: "\<lbrakk>is_root p\<rbrakk> \<Longrightarrow> path_from_root p [p]" |
-  PFRNode: "\<lbrakk>tree_topology; is_parent_of p q; path_from_root q as; distinct (as @ [p])\<rbrakk> \<Longrightarrow> path_from_root p (as @ [p])"
 
 lemma path_from_root_rev:
   assumes "path_from_root p ps"
@@ -3211,9 +2807,6 @@ lemma paths_eq:
   shows "(\<exists>ps. path_from_root p ps) = (\<exists>qs. path_to_root p qs)"
   using path_from_to path_to_from by blast
 
-inductive path_from_to :: "'peer \<Rightarrow> 'peer \<Rightarrow> 'peer list \<Rightarrow> bool" where
-  path_refl: "\<lbrakk>tree_topology; p \<in> \<P>\<rbrakk> \<Longrightarrow> path_from_to p p [p]" |
-  path_step: "\<lbrakk>tree_topology; is_parent_of p q; path_from_to r q as; distinct (as @ [p])\<rbrakk> \<Longrightarrow> path_from_to r p (as @ [p])"
 
 lemma path_from_to_rev:
   assumes "path_from_to r p r2p"
@@ -3413,13 +3006,6 @@ qed
 
 subsection "Influenced Language"
 
-(*fixed: without projection to p and q to the sends of w', the influenced language 
-is only correct if each node sends to exactly one child
-side note: proj. only needed in w', since by tree topology, each node p has a unique parent, and thus the receives 
-in w can already only be between p and q (i.e. the projection can be added for w as well but is unnecessary)*)
-inductive is_in_infl_lang :: "'peer \<Rightarrow> ('information, 'peer) action word \<Rightarrow> bool" where
-  IL_root: "\<lbrakk>is_root r; w \<in> \<L>(r)\<rbrakk> \<Longrightarrow> is_in_infl_lang r w" | \<comment>\<open>influenced language of root r is language of r\<close>
-  IL_node: "\<lbrakk>tree_topology; is_parent_of p q; w \<in> \<L>(p); is_in_infl_lang q w'; ((w\<down>\<^sub>?)\<down>\<^sub>!\<^sub>?) = (((w'\<down>\<^sub>{\<^sub>p\<^sub>,\<^sub>q\<^sub>})\<down>\<^sub>!)\<down>\<^sub>!\<^sub>?)\<rbrakk> \<Longrightarrow> is_in_infl_lang p w" \<comment>\<open>p is any node and q its parent has a matching send for each of p's receives\<close>
 
 lemma is_in_infl_lang_rev_tree:
   assumes "is_in_infl_lang p w" 
@@ -3451,18 +3037,6 @@ lemma child_matching_word_impl_in_infl_lang:
   assumes "tree_topology" and "is_parent_of p q" and "w \<in> \<L>(q)" and "is_in_infl_lang q w" and  "((w'\<down>\<^sub>?)\<down>\<^sub>!\<^sub>?) = (((w\<down>\<^sub>{\<^sub>p\<^sub>,\<^sub>q\<^sub>})\<down>\<^sub>!)\<down>\<^sub>!\<^sub>?)" and "w' \<in> \<L>(p)"
   shows "is_in_infl_lang p w'"
   using IL_node assms(1,2,4,5,6) by blast
-
-abbreviation InfluencedLanguage :: "'peer \<Rightarrow> ('information, 'peer) action language"  ("\<L>\<^sup>* _" [90] 100) where
-  "\<L>\<^sup>* p \<equiv> {w. is_in_infl_lang p w}"
-
-abbreviation InfluencedLanguageSend :: "'peer \<Rightarrow> ('information, 'peer) action language"  ("\<L>\<^sub>!\<^sup>* _" [90] 100) where
-  "\<L>\<^sub>!\<^sup>* p \<equiv> (\<L>\<^sup>* p)\<downharpoonright>\<^sub>! "
-
-abbreviation InfluencedLanguageRecv :: "'peer \<Rightarrow> ('information, 'peer) action language"  ("\<L>\<^sub>?\<^sup>* _" [90] 100) where
-  "\<L>\<^sub>?\<^sup>* p \<equiv> (\<L>\<^sup>* p)\<downharpoonright>\<^sub>? "
-
-abbreviation ShuffledInfluencedLanguage :: "'peer \<Rightarrow> ('information, 'peer) action language" ("\<L>\<^sup>*\<^sub>\<squnion>\<^sub>\<squnion> _" [90] 100) where
-  "\<L>\<^sup>*\<^sub>\<squnion>\<^sub>\<squnion> p \<equiv> shuffled_lang (\<L>\<^sup>* p)"
 
 lemma is_in_infl_lang_rev2: 
   assumes "w \<in> \<L>\<^sup>* p" and "is_node p"
@@ -3552,7 +3126,7 @@ lemma language_shuffle_subset :
 lemma shuffled_infl_lang_rev :
   assumes "v \<in> \<L>\<^sup>*(p)"
   shows "\<exists>v'. ( v' \<squnion>\<squnion>\<^sub>? v \<and> v' \<in> \<L>\<^sup>*\<^sub>\<squnion>\<^sub>\<squnion>(p))"
-  using assms by (rule CommunicatingAutomata.valid_input_shuffles_of_lang)
+  using assms by (rule valid_input_shuffles_of_lang)
 
 lemma shuffled_infl_lang_impl_valid_shuffle :
   assumes "v \<in> \<L>\<^sup>*\<^sub>\<squnion>\<^sub>\<squnion>(p)" 
@@ -3653,13 +3227,10 @@ lemma shuffle_origin:
 lemma shuffle_keeps_outputs_right:
   assumes "w' \<squnion>\<squnion>\<^sub>? (w)" and "is_output (last w)" 
   shows "is_output (last w')" 
-  using assms CommunicatingAutomata.shuffle_keeps_outputs_right_shuffled by metis
+  using assms shuffle_keeps_outputs_right_shuffled by metis
 
 
 
-\<comment> \<open>p receives from no one and there is no q that sends to p\<close>
-abbreviation no_sends_to_or_recvs_in :: "'peer \<Rightarrow> bool"  where
-  "no_sends_to_or_recvs_in p \<equiv> (\<P>\<^sub>?(p) = {} \<and> (\<forall>q. p \<notin> \<P>\<^sub>!(q)))"
 
 
 lemma root_graph: 
@@ -3836,12 +3407,6 @@ qed
 
 subsubsection "simulate sync with mbox word"
 
-\<comment> \<open>for each sending action, add the matching receive action directly after it\<close>
-fun add_matching_recvs :: "('information, 'peer) action word \<Rightarrow> ('information, 'peer) action word" where
-  "add_matching_recvs [] = []" |
-  "add_matching_recvs (a # w) = (if is_output a
-      then a # (?\<langle>get_message a\<rangle>) # add_matching_recvs w 
-      else a # add_matching_recvs w)"
 
 lemma add_matching_recvs_app : 
   shows "add_matching_recvs (xs \<cdot> ys) = (add_matching_recvs xs) \<cdot> (add_matching_recvs ys)"
@@ -3993,26 +3558,6 @@ lemma empty_sync_run_to_mbox_run :
 
 
 subsubsection "Lemma 4.4 and preparations"
-
-
-(*this should do the same thing as concat_infl but more straightforward *)
-inductive acc_infl_lang_word :: "'peer \<Rightarrow> ('information, 'peer) action word \<Rightarrow> bool" where
-  ACC_root: "\<lbrakk>is_root r; w \<in> \<L>\<^sup>*(r)\<rbrakk> \<Longrightarrow> acc_infl_lang_word r w" | \<comment>\<open>influenced language of root r is language of r\<close>
-  ACC_node: "\<lbrakk>tree_topology; is_parent_of p q; w \<in> \<L>\<^sup>*(p); acc_infl_lang_word q w'; ((w\<down>\<^sub>?)\<down>\<^sub>!\<^sub>?) = (((w'\<down>\<^sub>{\<^sub>p\<^sub>,\<^sub>q\<^sub>})\<down>\<^sub>!)\<down>\<^sub>!\<^sub>?)\<rbrakk> \<Longrightarrow> acc_infl_lang_word p (w' @ w)" \<comment>\<open>p is any node and q its parent has a matching send for each of p's receives\<close>
-
-
-
-
-
-
-
-
-
-(*starts at some node and a full path from that node to root, then walks up to the root while accumulating the word w1....wn*)
-inductive concat_infl :: "'peer \<Rightarrow> ('information, 'peer) action word \<Rightarrow> 'peer list  \<Rightarrow> ('information, 'peer) action word \<Rightarrow> bool" for p::"'peer" and w:: "('information, 'peer) action word" where
-  at_p: "\<lbrakk>tree_topology; w \<in> \<L>\<^sup>*(p); path_to_root p ps\<rbrakk> \<Longrightarrow> concat_infl p w ps w" | (*start condition*)
-  reach_root: "\<lbrakk>is_root q; qw \<in> \<L>\<^sup>*(q); path_to_root x (x # [q]); (\<forall>g. w_acc\<down>\<^sub>g \<in> \<L>\<^sup>*(g));  concat_infl p w (x # [q]) w_acc; (((w_acc\<down>\<^sub>x)\<down>\<^sub>?)\<down>\<^sub>!\<^sub>?) = (((qw\<down>\<^sub>{\<^sub>x\<^sub>,\<^sub>q\<^sub>})\<down>\<^sub>!)\<down>\<^sub>!\<^sub>?)\<rbrakk> \<Longrightarrow> concat_infl p w [q] (qw \<cdot> w_acc)" | (*end condition*)
-  node_step: "\<lbrakk>tree_topology; \<P>\<^sub>?(x) = {q}; (\<forall>g. w_acc\<down>\<^sub>g \<in> \<L>\<^sup>*(g)); path_to_root x (x # q # ps); qw \<in> \<L>\<^sup>*(q); concat_infl p w (x # q # ps) w_acc; (((w_acc\<down>\<^sub>x)\<down>\<^sub>?)\<down>\<^sub>!\<^sub>?) = (((qw\<down>\<^sub>{\<^sub>x\<^sub>,\<^sub>q\<^sub>})\<down>\<^sub>!)\<down>\<^sub>!\<^sub>?)\<rbrakk> \<Longrightarrow> concat_infl p w (q#ps) (qw \<cdot> w_acc)" 
 
 lemma concat_infl_path_rev :
   assumes "concat_infl p w (q#ps) w'"
@@ -4359,26 +3904,6 @@ lemma subword_of_sync_is_receivable2:
 
 section "new formalization"
 
-(*all receives possible in Aq, after performing actions in w*)
-abbreviation possible_recv_suffixes :: "('information, 'peer) action word \<Rightarrow> 'peer \<Rightarrow>  ('information, 'peer) action language"  ("\<ddagger>_\<ddagger>\<^sub>_" [90, 90] 110) where  
-  "\<ddagger>w\<ddagger>\<^sub>p \<equiv> {x\<down>\<^sub>? | x. (w \<cdot> x) \<in> \<L>\<^sup>*(p)}"
-
-(*all possible sends from q to p in Aq, after performing actions in w
-if p is not child of q, the set is trivially {\<epsilon>}*)
-abbreviation possible_send_suffixes_to_peer :: "'peer \<Rightarrow> ('information, 'peer) action word \<Rightarrow> 'peer \<Rightarrow>  ('information, 'peer) action language"  ("\<^sub>_\<ddagger>_\<ddagger>\<^sub>_" [90, 90, 90] 110) where  
-  "\<^sub>q\<ddagger>w\<ddagger>\<^sub>p \<equiv> {(x\<down>\<^sub>!)\<down>\<^sub>{\<^sub>p\<^sub>,\<^sub>q\<^sub>} | x. (w \<cdot> x) \<in> \<L>\<^sup>*(q)}"
-
-(*for all words w in p, for all w' that provide all the sends for the receives in w,
-w must be able to receive anything that q might send after performing w'.
-
-(there must be at least one such w' per w, otherwise w is not in the influenced language of p)*)
-definition subset_condition :: "'peer \<Rightarrow> 'peer \<Rightarrow> bool"
-  where "subset_condition p q \<longleftrightarrow> (\<forall> w \<in> \<L>\<^sup>*(p). \<forall> w' \<in> \<L>\<^sup>*(q).
-  (((w'\<down>\<^sub>!)\<down>\<^sub>{\<^sub>p\<^sub>,\<^sub>q\<^sub>})\<down>\<^sub>!\<^sub>? = ((w\<down>\<^sub>?)\<down>\<^sub>!\<^sub>?)) \<longrightarrow> ((\<^sub>q\<ddagger>w'\<ddagger>\<^sub>p)\<downharpoonright>\<^sub>!\<^sub>? \<subseteq> (\<ddagger>w\<ddagger>\<^sub>p)\<downharpoonright>\<^sub>!\<^sub>? ))"
-
-(*for all parent-child pairs, subset condition and shuffled language condition hold*)
-definition theorem_rightside :: "bool"
-  where "theorem_rightside \<longleftrightarrow> (\<forall>p \<in> \<P>. \<forall>q \<in> \<P>. ((is_parent_of p q) \<longrightarrow> ((subset_condition p q) \<and> ((\<L>\<^sup>*(p)) = (\<L>\<^sup>*\<^sub>\<squnion>\<^sub>\<squnion>(p)))) ))"
 
 lemma prefix_mbox_trace_valid:
   assumes "(w@v) \<in> \<L>\<^sub>\<infinity>"
@@ -4732,7 +4257,7 @@ than in v', it must also be sent earlier in e, contradicting that they have the 
 \<and> e \<in> \<T>\<^bsub>None\<^esub> \<and> ?v' \<in> \<T>\<^bsub>None\<^esub> \<and> (v \<cdot> [a]) \<in> \<T>\<^bsub>None\<^esub>\<downharpoonright>\<^sub>! \<and> ?v' = (add_matching_recvs v) \<and> ?v'\<down>\<^sub>q \<in> \<L>\<^sup>* q
 \<and> ?wq \<in> \<L>\<^sup>* q" 
         by (metis (no_types, lifting) False Suc.prems(1) \<open>(a # \<epsilon>)\<down>\<^sub>q = a # \<epsilon>\<close> \<open>(wq \<cdot> xs)\<down>\<^sub>! = wq\<down>\<^sub>!\<close>
-            \<open>(wq \<cdot> xs)\<down>\<^sub>? = (add_matching_recvs v \<cdot> a # \<epsilon>)\<down>\<^sub>q\<down>\<^sub>?\<close> \<open>add_matching_recvs v\<down>\<^sub>q \<cdot> a # \<epsilon> \<noteq> wq \<cdot> xs\<close>
+            \<open>((wq \<cdot> xs)\<down>\<^sub>?) = ((add_matching_recvs v \<cdot> a # \<epsilon>)\<down>\<^sub>q)\<down>\<^sub>?\<close> \<open>add_matching_recvs v\<down>\<^sub>q \<cdot> a # \<epsilon> \<noteq> wq \<cdot> xs\<close>
             \<open>add_matching_recvs v\<down>\<^sub>q \<in> \<L>\<^sup>* q\<close> e_def filter_append v'a1 v_IH w_def wq_to_v'a_trace wqxs_L)
 
       have "(e \<cdot> xs) \<in> \<T>\<^bsub>None\<^esub>" using exec_append_missing_recvs[of wq xs r q v a e]  using diff_trace_prems wq_def wqxs_trace_match 
@@ -4789,18 +4314,6 @@ lemma matched_mbox_run_to_sync_run :
 
 subsection "=> 1. "
 
-(*mix some w' of L*(Aq) with matching w of L*(Ap) s.t. each send in q (to p!) is directly followed
-by the matching send. The order of the peer words in the result word is kept*)
-fun mix_pair :: "('information, 'peer) action word \<Rightarrow> ('information, 'peer) action word \<Rightarrow> ('information, 'peer) action word \<Rightarrow> ('information, 'peer) action word" where
- "mix_pair [] [] acc = acc" |
- "mix_pair (a # w') [] acc = mix_pair w' [] (a # acc)" |
- "mix_pair [] (a # w) acc = mix_pair [] w (a # acc)" |
- "mix_pair (a # w') (b # w) acc  = (if a = !\<langle>get_message b\<rangle>
-      then (if b = ?\<langle>get_message a\<rangle> then mix_pair w' w (a # b # acc) else mix_pair (a # w') w (b # acc))
-      else mix_pair w' (b # w) (a # acc))"
-
-
-
 
 subsection "=> 2."
 
@@ -4811,11 +4324,6 @@ and "is_output b" and "is_input a" and "v = xs \<cdot> b # a # ys"
 shows "\<exists> as bs. vq\<down>\<^sub>!\<down>\<^sub>{\<^sub>p\<^sub>,\<^sub>q\<^sub>} = (as\<down>\<^sub>!\<down>\<^sub>{\<^sub>p\<^sub>,\<^sub>q\<^sub>} \<cdot> (!\<langle>get_message a\<rangle>) # bs\<down>\<^sub>!\<down>\<^sub>{\<^sub>p\<^sub>,\<^sub>q\<^sub>})"
   sorry
 
-(*construction: do mix_pair until k is reached, for k and k+1 instead put vq's send and then both v!k and v!(k+1) and then continue with mix_pair construction*)
-inductive mix_shuf :: "('information, 'peer) action word \<Rightarrow> ('information, 'peer) action word \<Rightarrow> ('information, 'peer) action word \<Rightarrow> ('information, 'peer) action word \<Rightarrow> bool" where  
-  mix_shuf_constr: "\<lbrakk>vq\<down>\<^sub>!\<down>\<^sub>{\<^sub>p\<^sub>,\<^sub>q\<^sub>}\<down>\<^sub>!\<^sub>? = v\<down>\<^sub>?\<down>\<^sub>!\<^sub>?; v' \<in> \<L>\<^sup>*\<^sub>\<squnion>\<^sub>\<squnion>(p); v' \<squnion>\<squnion>\<^sub>? v; v \<in> \<L>\<^sup>*(p); vq \<in> \<L>\<^sup>*(q); 
-vq = (as \<cdot> a_send # bs); v = xs \<cdot> b # a_recv # ys; get_message a_recv = get_message a_send; is_input a_recv; is_output a_send; is_output b\<rbrakk> 
-\<Longrightarrow> mix_shuf vq v v' ((mix_pair as xs []) \<cdot> a_send # b # a_recv # (mix_pair bs ys []))"
 
 
 (*
